LambdaLab.lean
@@ -1,6 +1,7 @@
 -- This module serves as the root of the `LambdaLab` library.
 -- Import modules here that should be built as part of the library.
-import LambdaLab.Relation.Basic
+import LambdaLab.Relation.Closure
+import LambdaLab.Relation.Normalization
 import LambdaLab.Stlc.DeBruijn.Basic
 import LambdaLab.Stlc.DeBruijn.Typing
 import LambdaLab.Stlc.DeBruijn.Step
